reflect latest changes

examples/ping/interfaces.v
@@ -1,7 +1,7 @@
 From monae Require Import preamble hierarchy.
 From Stdlib Require Import Lia.
 
-From mathcomp Require Import ssreflect ssrbool eqtype ssrfun seq.
+From mathcomp Require Import ssreflect ssrbool eqtype ssrfun seq ssrnat.
 From FreerDPS Require Import Core HoareFacts.
 
 Set Implicit Arguments.
@@ -10,30 +10,30 @@ Unset Printing Implicit Defensive.
 
 Local Obligation Tactic := simpl.
 
-Generalizable All Variables. 
+Generalizable All Variables.
 Local Open Scope monae_scope.
 Import FreerFuns.
 
 Create HintDb ping_db.
 
 (**
-  * We consider : 
-  * - a client C (contract) ;
-  * - a server S (contract) ;
-  * - and a network N (lossy channel). 
-  *)
+* We consider :
+* - a client C (contract) ;
+* - a server S (contract) ;
+* - and a network N (lossy channel).
+*)
 
 (**
-  * Client sends a PING packet to the server 
-  * through network then waits for PONG as 
-  * response.
-  *)
+* Client sends a PING packet to the server
+* through network then waits for PONG as
+* response.
+*)
 
 (**
-  * Server repeatedly waits for a PING packet 
-  * from the network then sends a PONG as 
-  * response.
-  *)
+* Server repeatedly waits for a PING packet
+* from the network then sends a PONG as
+* response.
+*)
 
 (* ======================================================================== *)
 
@@ -44,8 +44,8 @@ Inductive M := ping | pong.
 (* ======================================================================== *)
 
 (* Client is described as :
- * C = send (ping); wait (pong).
- *)
+* C = send (ping); wait (pong).
+*)
 Inductive client_api : effect :=
 | SEND : M -> client_api unit
 | WAIT : client_api M.
@@ -56,19 +56,20 @@ Definition wait `{Provide ix client_api} {im : freerMonad ix} : im M :=
   trigger (im:=im) (inj_p $ WAIT).
 
 Definition C `{Provide ix client_api} {im : freerMonad ix} : im M :=
-  send >> wait.
+  send >>= fun=> wait.
 
 (* ======================================================================== *)
 
 Fixpoint loop `{Provide ix i} {im : freerMonad ix} (fuel : nat) `(prog : im X)
-    : im unit := match fuel with
+  : im unit :=
+match fuel with
 | 0%nat => prog >> skip
 | S ful => prog >> loop ful prog
 end.
 
 (* Server is described as :
- * S = μX. recv(ping); reply(pong); X.
- *)
+* S = μX. recv(ping); reply(pong); X.
+*)
 Inductive server_api : effect :=
 | RPLY : M -> server_api unit
 | RECV : server_api M.
@@ -81,9 +82,10 @@ Definition recv `{Provide ix server_api} {im : freerMonad ix} : im M :=
 Definition S_p `{Provide ix server_api} {im : freerMonad ix} : im unit :=
   recv >> reply.
 Definition S_ `{Provide ix server_api} {im : freerMonad ix} (fuel : nat)
-    : im unit := loop fuel S_p.
+  : im unit :=
+loop fuel S_p.
 
- 
+
 (* ======================================================================== *)
 
 Module NetworkChannelMod.
@@ -98,14 +100,16 @@ Record N := mk_chan {
 
 Definition send_over_network (m : M) (n : N) :=
   {| tx := m :: tx n; rx := rx n |}.
-Definition consume_received (n : N) := match rx n with
+
+Definition consume_received (n : N) :=
+match rx n with
 | [::] => {| tx := tx n ; rx := [::] |}
 | _ :: ns => {| tx := tx n ; rx := ns |}
-end.  
+end.
 
 Fact consuming_has_no_effect_on_tx : forall n, tx (consume_received n) = tx n.
 Proof.
-  by move => n; rewrite /consume_received; case : (rx n).
+  by move => n; rewrite /consume_received; case: (rx n).
 Qed.
 
 End NetworkChannelMod.
@@ -115,200 +119,189 @@ Import NetworkChannelMod.
 (* ======================================================================== *)
 
 (* Contracts *)
-      Local Open Scope nat_scope.
+Local Open Scope nat_scope.
 
 Module ccm.
-  Section ccs.
-    (* make_contract
-     : forall (i : effect) (Ω : UU0),
+Section ccs.
+(* make_contract
+: forall (i : effect) (Ω : UU0),
 (Ω -> forall α : UU0, i α -> α -> Ω) ->
 (Ω -> forall α : UU0, i α -> Prop) ->
 (Ω -> forall α : UU0, i α -> α -> Prop) -> contract i Ω *)
 
-      Definition c_step (network : N) : forall X, client_api X -> X -> N :=
-        fun X ec x =>
-          match ec with
-          | SEND m => send_over_network m network
-            (* add packet tx *)
-          | WAIT => consume_received network
-            (* remove packet rx (if present) *)
-          end.
+Definition c_step (network : N) : forall X, client_api X -> X -> N :=
+fun X ec x =>
+match ec with
+| SEND m => send_over_network m network
+  (* add packet tx *)
+| WAIT => consume_received network
+  (* remove packet rx (if present) *)
+end.
 
-      Inductive c_o_caller (st : N) : forall X, client_api X -> Prop :=
-      | O_WAIT (equ : forall ns, ping :: ns = st.(tx)) : c_o_caller st WAIT
-      | O_SEND (m : M) : c_o_caller st (SEND m)
-      .
-      Hint Constructors c_o_caller : ping_db.
+Inductive c_o_caller (st : N) : forall X, client_api X -> Prop :=
+| O_WAIT (equ : forall ns, ping :: ns = st.(tx)) : c_o_caller st WAIT
+| O_SEND (m : M) : c_o_caller st (SEND m)
+.
 
-    Check head.
-    (* Search (seq _ -> ) *)
-      Inductive c_o_callee (st : N) : forall X, client_api X -> X -> Prop :=
-      | SEND_O (u : unit) (m : M) (equ_m : m = ping)
-          (equ : forall ns, m :: ns = st.(tx)) : c_o_callee st (SEND m) u
-      | WAIT_O : c_o_callee st WAIT pong
-      (* | WAIT_O (m : M) (msg_output : m = pong)
-           (equ : first_not_from_me from st) : c_o_callee from to st WAIT m *)
-      (* | SEND_O (u : unit) (equ : Some ping = (peek_first st).(message))
-           : c_o_callee from to st (SEND ping) u *)
-      .
-      Hint Constructors c_o_callee : ping_db.
+Inductive c_o_callee (st : N) : forall X, client_api X -> X -> Prop :=
+| SEND_O (u : unit) (m : M) (equ_m : m = ping)
+  (equ : forall ns, m :: ns = st.(tx)) : c_o_callee st (SEND m) u
+| WAIT_O : c_o_callee st WAIT pong.
 
-      Definition c_contract :=
-        make_contract c_step no_caller_obligation c_o_callee.
+Definition c_contract :=
+make_contract c_step no_caller_obligation c_o_callee.
 
-      (* Safety *)
-      Lemma c_respect `{Provide ix client_api} {im : freerMonad ix}
-          (network : N)
-        : pre (to_hoare (im:=im) c_contract C) network.
-      (*
-      Proof.
-        prove impure with ping_db.
-      Qed.
-      *)
-      Admitted.
+(* Safety *)
+Lemma c_respect `{Provide ix client_api} {im : freerMonad ix} (network : N)
+  : pre (to_hoare (im:=im) c_contract C) network.
+Proof.
+by apply/to_hoare_bind_preI=> [|??];
+  rewrite to_hoare_request_preE /gen_caller_obligation proj_inj_p_equ.
+Qed.
 
-      (* Liveness *)
-      Lemma c_run `{Provide ix client_api} {im : freerMonad ix}
-          (initial_network final_network : N) (m : M)
-        (run : post (to_hoare (im:=im) c_contract C)
-          initial_network m final_network)
-        : m = pong.
-      (*
-      Proof.
-        (* Tactic `unroll_post` needs to be reworked automatically. *)
-        by run_simpl run;
-          cleanvert H1;
-          simplify_gens;
-          destruct run as [wait_callee wait_state];
-          simplify_gens;
-          inversion wait_callee; subst;
-          cleanvert wait_state; cleanvert H1; cleanvert H2; cleanvert H3;
-          simplify_gens;
-          cleanvert H1.
-      Qed.
-      *)
-      Admitted.
-  End ccs.
+(* Liveness *)
+Lemma wait_postE `{Provide ix client_api} (network final_network : N) (m : M) :
+  post (to_hoare (im:=freer ix) c_contract wait) network m final_network ->
+  m = pong.
+Proof.
+rewrite to_hoare_request_postE /gen_witness_update /gen_callee_obligation !proj_inj_p_equ /=.
+by move=> [_ wait]; inversion wait; ssubst.
+Qed.
+
+Lemma c_run `{Provide ix client_api} {im : freerMonad ix} (initial_network final_network : N) (m : M)
+    (run : post (to_hoare (im:=freer ix) c_contract C) initial_network m final_network)
+  : m = pong.
+Proof.
+move: run; rewrite to_hoare_bind_postE.
+by move=> -[? [? [_ +]]]=> /wait_postE.
+Qed.
+
+(* TODO: Don't forget you need to look at an example for
+  equational reasoning from monae's 2025 paper. *)
+End ccs.
 End ccm.
 
 (* ------------------------------------------------------------------------ *)
 
 
 Module scm.
-  Section scs.
+Section scs.
 
 
-      Definition s_step (network : N) : forall X, server_api X -> X -> N :=
-        fun X ec x =>
-          match ec with
-          | RPLY m => send_over_network m network
-          | RECV => consume_received network
-          end.
+Definition s_step (network : N) : forall X, server_api X -> X -> N :=
+fun X ec x =>
+match ec with
+| RPLY m => send_over_network m network
+| RECV => consume_received network
+end.
 
-      Inductive s_o_caller (st : N) : forall X, server_api X -> Prop :=
-      | O_RECV (*blocking : rx st <> [::]*) : s_o_caller st RECV
-      | O_RPLY (m : M) : s_o_caller st (RPLY m)
-      .
-      Hint Constructors s_o_caller : ping_db.
+Inductive s_o_caller (st : N) : forall X, server_api X -> Prop :=
+| O_RECV (*blocking : rx st <> [::]*) : s_o_caller st RECV
+| O_RPLY (m : M) : s_o_caller st (RPLY m)
+.
+Hint Constructors s_o_caller : ping_db.
 
-      Inductive s_o_callee (st : N) : forall X, server_api X -> X -> Prop :=
-      | RECV_O (m : M) : s_o_callee st RECV ping
-      | RPLY_O (u : unit) (m : M) : s_o_callee st (RPLY m) u
-      .
-      Hint Constructors s_o_callee : ping_db.
+Inductive s_o_callee (st : N) : forall X, server_api X -> X -> Prop :=
+| RECV_O (m : M) : s_o_callee st RECV ping
+| RPLY_O (u : unit) (m : M) : s_o_callee st (RPLY m) u
+.
+Hint Constructors s_o_callee : ping_db.
 
-      Definition s_contract := make_contract s_step s_o_caller s_o_callee.
+Definition s_contract := make_contract s_step s_o_caller s_o_callee.
 
+Lemma recv_postE `{Provide ix server_api} {im : freerMonad ix}
+    (network final_network : N) (m : M) :
+  post (to_hoare (im:=im) s_contract recv) network m final_network ->
+  m = ping /\ final_network = consume_received network.
+Proof.
+rewrite /recv to_hoare_request_postE /gen_witness_update.
+rewrite /gen_callee_obligation proj_inj_p_equ /=.
+move=> [-> recv_result].
+inversion recv_result; ssubst.
+by [].
+Qed.
 
-      Lemma s_respect `{Provide ix server_api} {im : freerMonad ix}
-          (network : N) fuel
-        : pre (to_hoare (im:=im) s_contract (S_ fuel)) network.
-      (*
-      Proof.
-        move : network;
-          elim : fuel => [|ful EH] network;
-          prove impure with ping_db; constructor.
-      Qed.
-      *)
-      Admitted.
+Lemma reply_postE `{Provide ix server_api} {im : freerMonad ix}
+    (network final_network : N) (u : unit) :
+  post (to_hoare (im:=im) s_contract reply) network u final_network ->
+  final_network = send_over_network pong network.
+Proof.
+rewrite /reply to_hoare_request_postE /gen_witness_update.
+rewrite /gen_callee_obligation proj_inj_p_equ /=.
+by move=> [-> _].
+Qed.
 
-      Lemma s_p_run_grows `{Provide ix server_api} {im : freerMonad ix}
-          (initial_network final_network : N) (u : unit)
-        (run : post (to_hoare (im:=im) s_contract S_p)
-          initial_network u final_network)
-        : tx final_network = pong :: tx initial_network.
-      (*
-      Proof.
-        (* Should be :
-        by unroll_post run;
-          rewrite /= consuming_has_no_effect_on_tx.
-        *)
-        by run_simpl run;
-          cleanvert H1;
-          simplify_gens;
-          run_simpl run;
-          case : run => [reply_callee reply_state];
-          simplify_gens;
-          inversion reply_callee; subst;
-          cleanvert reply_state; cleanvert H1; cleanvert H2; cleanvert H3;
-          simplify_gens; cleanvert H1;
-          rewrite /= consuming_has_no_effect_on_tx.
-      Qed.
-      *)
-      Admitted.
+Import SpecializedHoareModule.
 
-      Lemma s_run `{Provide ix server_api} {im : freerMonad ix}
-          (initial_network final_network : N) (u : unit) fuel
-        (run : post (to_hoare (im:=im) s_contract (S_ fuel))
-          initial_network u final_network)
-        : tx final_network = nseq (S fuel) pong ++ tx initial_network.
-      (*
-      Proof.
-        move : initial_network final_network u run.
-        elim : fuel => [|fuel IH] initial_network final_network u.
-        - (* Should be : by unroll_post; rewrite (s_p_run_grows run_p). *)
-          by move => /(to_hoare_post_bind_assoc s_contract
-            (S_p (im:=ImpureModule_acto__canonical__Impure_MonadImpure ix))
-            (fun _ : unit =>
-              skip (M:=ImpureModule_acto__canonical__Impure_MonadImpure ix)))
-            [x [middle_network [run_p run_skip]]];
-            run_simpl run_skip;
-            rewrite (s_p_run_grows run_p).
-        move=> /(to_hoare_post_bind_assoc s_contract
-          (S_p (im:=ImpureModule_acto__canonical__Impure_MonadImpure ix))
-          (fun _ : unit =>
-            S_ (im:=ImpureModule_acto__canonical__Impure_MonadImpure ix) fuel))
-            [x [middle_network [run_p run_loop]]];
-            rewrite /= (IH _ _ _ run_loop) (s_p_run_grows run_p) //;
-            clear IH run_loop run_p.
+Lemma s_p_respect `{Provide ix server_api} {im : freerMonad ix}
+    (network : N) :
+  pre (to_hoare (im:=im) s_contract S_p) network.
+Proof.
+by apply/to_hoare_bind_preI=> [|??];
+  rewrite to_hoare_request_preE /gen_caller_obligation proj_inj_p_equ;
+  constructor.
+Qed.
 
-        have nseq_pong_cons : forall n,
-          nseq n pong ++ pong :: tx initial_network =
-          nseq (S n) pong ++ tx initial_network by
-            by elim => [|n IHn] //=; rewrite IHn.
+Lemma s_respect `{Provide ix server_api}
+(network : N) fuel
+: pre (to_hoare (im:=freer ix) s_contract (S_ fuel)) network.
+Proof.
+move: network; elim: fuel=> [|n ih] network;
+  apply/to_hoare_bind_preI=> [|??].
+- exact/s_p_respect.
+- by move=>_; apply/to_hoare_skip_preI.
+- exact/s_p_respect.
+- by move=>?; apply/ih.
+Qed.
 
-        exact: nseq_pong_cons.
-      Qed.
-      *)
-      Admitted.
+Lemma s_p_run_grows `{Provide ix server_api} {im : freerMonad ix}
+(initial_network final_network : N) (u : unit)
+(run : post (to_hoare (im:=im) s_contract S_p)
+initial_network u final_network)
+: tx final_network = pong :: tx initial_network.
+Proof.
+move: run; rewrite to_hoare_bind_postE=> -[received [net [recv_run reply_run]]].
+move: reply_run recv_run
+  => /reply_postE ->
+  => /recv_postE [_ ->].
+by rewrite /= consuming_has_no_effect_on_tx.
+Qed.
 
-      Lemma s_run_size `{Provide ix server_api} {im : freerMonad ix}
-          (initial_network final_network : N) (u : unit) fuel
-        (run : post (to_hoare (im:=im) s_contract (S_ fuel))
-          initial_network u final_network)
-        : size (tx final_network) = size (tx initial_network) + fuel + 1.
-      (*
-      Proof.
-        have -> : tx final_network = nseq (S fuel) pong ++ tx initial_network
-          := s_run (im:=im) (initial_network:=initial_network)
-            (final_network:=final_network) (u:=u) (fuel:=fuel) run.
-        rewrite size_cat size_nseq;
-          lia.
-      Qed.
-      *)
-      Admitted.
+Lemma s_run `{Provide ix server_api}
+(initial_network final_network : N) (u : unit) fuel
+(run : post (to_hoare (im:=freer ix) s_contract (S_ fuel))
+initial_network u final_network)
+: tx final_network = nseq (S fuel) pong ++ tx initial_network.
+Proof.
+move: initial_network final_network u run.
+elim: fuel=> [|fuel IH] initial_network final_network u run.
+- move: run.
+  rewrite /S_ /loop to_hoare_bind_postE.
+  move=> [x [middle_network [run_p run_skip]]].
+  move: run_skip.
+  rewrite to_hoare_local_postE=> -[_ <-].
+  by rewrite /= (s_p_run_grows run_p).
+move: run.
+rewrite /S_ /loop to_hoare_bind_postE.
+move=> [x [middle_network [run_p run_loop]]].
+rewrite (IH _ _ _ run_loop) (s_p_run_grows run_p).
+have nseq_pong_cons : forall n,
+  nseq n pong ++ pong :: tx initial_network =
+  nseq (S n) pong ++ tx initial_network.
+  by elim=> [|n IHn] //=; rewrite IHn.
+exact: nseq_pong_cons.
+Qed.
 
-  End scs.
+Lemma s_run_size `{Provide ix server_api}
+(initial_network final_network : N) (u : unit) fuel
+(run : post (to_hoare (im:=freer ix) s_contract (S_ fuel))
+initial_network u final_network)
+: size (tx final_network) = size (tx initial_network) + fuel + 1.
+Proof.
+by rewrite (s_run run) size_cat size_nseq addSn addnC addn1.
+Qed.
+
+End scs.
 End scm.
 
 (* ------------------------------------------------------------------------ *)
@@ -319,10 +312,10 @@ Import ccm scm.
 
 (* Protocol description *)
 (**
-    Now, lets try to model this :
+Now, lets try to model this :
 
-(a)    +---+ ==> (1) send ping ==> +---+ ==> (2) dlvr ping ==> +---+ 
-       | C |                       | N |                       | S |
+(a)    +---+ ==> (1) send ping ==> +---+ ==> (2) dlvr ping ==> +---+
+| C |                       | N |                       | S |
 (b)    +---+ <== (4) dlvr pong <== +---+ <== (4) send pong <== +---+
 
 **)
@@ -335,28 +328,28 @@ Import ccm scm.
 (* Packet loss are independant. *)
 
 (** One single round for receiving a pong equals :
-  * P(pong_recv) = P (ping_del) * P (pong_del)
-  * P(pong_recv) = (1 - p) * (1 - p)
-  * P(pong_recv) = (1 - p)^2
-  *)
+* P(pong_recv) = P (ping_del) * P (pong_del)
+* P(pong_recv) = (1 - p) * (1 - p)
+* P(pong_recv) = (1 - p)^2
+*)
 
 (**
-  * For each retry, we get :
-  * q = (1 - p)^2
-  *)
+* For each retry, we get :
+* q = (1 - p)^2
+*)
 
 (**
-  * For at most n attempts, we get :
-  * P(n) = 1 - (1 - q)^n = 1 - (1 
-  - [1 - p]^2)^n
-  *)
+* For at most n attempts, we get :
+* P(n) = 1 - (1 - q)^n = 1 - (1
+- [1 - p]^2)^n
+*)
 
-(** 
-  * composing with quasi assoc
-  * s.~ = p.~ * q.~ = p + (p.~ * q) <== this is the good equiv
-  * 1 - ((1 - p) * (1 - q)) = p + ((1 - p) * q)
-  * 1 - (1 - q - (p - pq)) = p + (q - pq)
-  * 1 - (1 - q - p + pq) = p + q - pq
-  * 1 - 1 + q + p - pq = p + q - pq
-  * 0 + q + p - pq = p + q - pq
-  *)
+(**
+* composing with quasi assoc
+* s.~ = p.~ * q.~ = p + (p.~ * q) <== this is the good equiv
+* 1 - ((1 - p) * (1 - q)) = p + ((1 - p) * q)
+* 1 - (1 - q - (p - pq)) = p + (q - pq)
+* 1 - (1 - q - p + pq) = p + q - pq
+* 1 - 1 + q + p - pq = p + q - pq
+* 0 + q + p - pq = p + q - pq
+*)
